\qitem{%
    Let $p$ be an odd prime, then
    \begin{alignat*}{1}
        \left(\left(\frac{p-1}{2}\right)!\right)^2\equiv (-1)^{\frac{p+1}{2}} (p)
    \end{alignat*}
    }{%
    \begin{alignat*}{1}
        \left(\left(\frac{p-1}{2}\right)!\right)^2&\equiv \frac{p-1}{2}! (p-1)(p-2)\cdots (p-\frac{p-1}{2})\cdot (-1)^{p-1/2}\\
                                                  &\equiv -1\cdot (-1)^{(p-1)/2}\\
                                                  &\equiv (-1)^{\frac{p+1}{2}} (p) 
    \end{alignat*}
    }{%
    <++>
}

