\pitem[]{%
    For $n\geq 1$, prove that
    \[
        \sum_{k=0}^{n}(-1)^k\binom{n}{k}=0.
    \]
    }{%
    Take the elements of $[n]$. Take the element $1$ (we know that $n\geq 1$). For every subset $S$ of $[n]$ with $k$ elements, where $k$ is even, we can get a unique subset with an odd number of elements as follows: if $1\in S$ remove it, otherwise, add it. And obviously, every subset with an odd number of element arise from this way. Hence there is a bijection between even subsets and odd subsets.
    }{%
    1.10
}
