\mysection{Arithmetic Mean - Geometric Mean}

\begin{mysubsection}{}
    \begin{theorem}[thm:]{AM-GM}
        For any real numbers $x_1, x_2, \ldots, x_n \geq 0$, \[\frac{x_1 + x_2 + \cdots + x_n}{n} \geq \sqrt[n]{x_1 x_2 \cdots x_n}\] with equality if and only if $x_1 = x_2 = \cdots = x_n$. 
    \end{theorem}
    \begin{proof}
        The arguement is based on Cauchy Induction, which is to prove that $s(2)$ is true, and that $s(n)$ implies $s(2n)$. This implies that $s(2^m)$ is true for all positive $m$. Then prove that $s(n)$ implies $s(n-1)$. Then $s(n)$ is true for all $n\geq 2$. 

        But the main idea is base on the following observation:
        \begin{alignat*}{1}
            \frac{a+b}{2}-\sqrt{ab}&= \frac{a+b-2\sqrt{ab}}{2} =\frac{1}{2} \left(\sqrt{a}-\sqrt{b}\right)^2\geq 0.
        \end{alignat*}
        The equality holds if and only if $\sqrt{a}-\sqrt{b}$, that is when $a=b$.
        %https://artofproblemsolving.com/wiki/index.php/Cauchy_Induction
    \end{proof}

    We can use AM-GM to gives us various results:
    \begin{enumerate}
        \item $1+x\geq 2\sqrt{x}$
        \item $x^2+y^2\geq 2xy$
        \item $\dfrac{a}{b}+\dfrac{b}{a}\geq 2$
        \item $ax+\dfrac{b}{x}\geq 2\sqrt{ab}$
    \end{enumerate}
\end{mysubsection}

\begin{shortque}[]{}
    \qitem{%
        For $x,y>0$, prove that $2(x^2+y^2)\geq (x+y)^2$.
        }{%
        We have $x^2+y^2\geq 2xy$, adding $x^2+y^2$ to both side, we have the result.
        }{%
        <++>
    }

    \qitem{%
        Find the maximum of $2 - a - \frac{1}{2a}$ for all positive $a$. 
        }{%
        We can rewrite the given expression as $2 - (a + \frac{1}{2a})$. To maximize the whole expression, we must minimize $a + \frac{1}{2a}$. Since $a$ is positive, so is $\frac{1}{2a}$. This means AM - GM will hold for $a$ and $\frac{1}{2a}$.

        By AM - GM, the arithmetic mean of $a$ and $\frac{1}{2a}$ is at least their geometric mean, or $\frac{\sqrt{2}}{2}$. This means the sum of $a$ and $\frac{1}{2a}$ is at least $\sqrt{2}$. We can prove that we can achieve this minimum for $a + \frac{1}{2a}$ by plugging in $a = \frac{\sqrt{2}}{2}$ by solving $a + \frac{1}{2a} = \sqrt{2}$ for $a$.

        Plugging in $a = \frac{\sqrt{2}}{2}$ into our original expression that we wished to maximize, we get that $2 - a - \frac{1}{2a} = \boxed{2 - \sqrt{2}}$, which is our answer. 
        }{%
        https://artofproblemsolving.com/wiki/index.php/Solution_to_AM_-_GM_Introductory_Problem_2
    }
\end{shortque}

